experiment/Experiment.Repr.Fun.fsti
@@ -1,0 +1,277 @@
+module Experiment.Repr.Fun
+
+module U  = Learn.Util
+module MP = FStar.Monotonic.Pure
+
+
+/// [tys] describes a family of types, indexed by [t]. Those types are used for the returned values of programs.
+/// - [v] map the index to the associated type
+/// - [r ty] is a "concrete" representation of [v ty]
+/// - [unit] should be associated to a type with an unique element [emp]
+/// - [all] and [ex] are representations of the universal and existential quantification. They are used when
+///   generating the VC. They must be equivalent to a quantification on [v ty]
+noeq
+type tys' = {
+  t : Type u#t;
+  v : t -> Type u#v;
+  r : t -> Type u#r;
+  v_of_r : (#ty : t) -> r ty -> v ty;
+  r_of_v : (#ty : t) -> v ty -> r ty;
+  unit : t;
+  emp  : v unit;
+  all  : (ty : t) -> (v ty -> Type0) -> Type0;
+  ex   : (ty : t) -> (v ty -> Type0) -> Type0; 
+}
+
+type tys = s : tys' {
+  (forall (ty : s.t) (x : s.v ty) . {:pattern (s.v_of_r (s.r_of_v x))} s.v_of_r (s.r_of_v x) == x) /\
+  (forall (x : s.v s.unit) . x == s.emp) /\
+  (forall (ty : s.t) (f : s.v ty -> Type0) . {:pattern (s.all ty f)} s.all ty f <==> (forall (x : s.v ty) . f x)) /\
+  (forall (ty : s.t) (f : s.v ty -> Type0) . {:pattern (s.ex  ty f)} s.ex  ty f <==> (exists (x : s.v ty) . f x))
+}
+
+let can_tys : tys u#(v+1) u#v u#v = {
+  t = Type u#v;
+  v = (fun ty -> ty);
+  r = (fun ty -> ty);
+  v_of_r = (fun x -> x);
+  r_of_v = (fun x -> x);
+  unit = U.unit';
+  emp  = U.Unit';
+  all  = (fun ty p -> forall (x : ty) . p x);
+  ex   = (fun ty p -> exists (x : ty) . p x)
+}
+
+noeq
+type prog_tree (#s : tys u#t u#v u#r) : s.t -> Type u#(max t v r a + 1) =
+  | Tnew   : (a : s.t) -> prog_tree #s a
+  | Tasrt  : (p : prop) -> prog_tree #s s.unit
+  | Tasum  : (p : prop) -> prog_tree #s s.unit
+  | Tspec  : (a : s.t) -> (pre : pure_pre) -> (post : pure_post (s.v a)) ->
+             prog_tree #s a
+  | Tret   : (a : s.t) -> (x : s.r a) -> prog_tree #s a
+  | Tbind  : (a : s.t) -> (b : s.t) ->
+             (f : prog_tree #s a) -> (g : s.v a -> prog_tree #s b) ->
+             prog_tree #s b
+  (* [a] could be of type [s.t] *)
+  | TbindP : (a : Type u#a) -> (b : s.t) ->
+             (wp : pure_wp a) -> (x : unit -> PURE a wp) -> (g : a -> prog_tree #s b) ->
+             prog_tree #s b
+
+unfold
+let return (#s : tys) (#a : s.t) ($x : s.v a) : prog_tree #s a
+  = Tret a (s.r_of_v x)
+
+unfold
+let bind (#s : tys) (#a #b : s.t) (f : prog_tree #s a) (g : s.v a -> prog_tree #s b) : prog_tree #s b
+  = Tbind a b f g
+
+
+(***** Shape *)
+
+type shape_tree : Type0 =
+  | Snew | Sasrt | Sasum | Sspec
+  | Sret   : (smp_ret : bool) -> shape_tree
+  | Sbind  : (f : shape_tree) -> (g : shape_tree) -> shape_tree
+  | SbindP : (g : shape_tree) -> shape_tree
+
+let rec prog_has_shape (#ts : tys) (#a : ts.t) (t : prog_tree u#t u#v u#r u#a #ts a) (s : shape_tree)
+  : Tot prop (decreases t)
+  = match t returns prop with
+  | Tnew _           -> s == Snew
+  | Tasrt _          -> s == Sasrt
+  | Tasum _          -> s == Sasum
+  | Tspec _ _ _      -> s == Sspec
+  | Tret  _ _        -> exists (smp_ret : bool) .
+                       s == Sret smp_ret
+  | Tbind a _ f g    -> exists (s_f s_g : shape_tree) .
+                       s == Sbind s_f s_g /\
+                       prog_has_shape f s_f /\
+                      (forall (x : ts.v a) . prog_has_shape (g x) s_g)
+  | TbindP a _ _ f g -> exists (s_g : shape_tree) .
+                       s == SbindP s_g /\
+                      (forall (x : a) . prog_has_shape (g x) s_g)
+
+let rec prog_has_shape' (#ts : tys) (#a : ts.t) (t : prog_tree u#t u#v u#r u#a #ts a) (s : shape_tree)
+  : Pure prop (requires True) (ensures fun p -> p <==> prog_has_shape t s) (decreases t)
+  = match t returns prop with
+  | Tnew _           -> s == Snew
+  | Tasrt _          -> s == Sasrt
+  | Tasum _          -> s == Sasum
+  | Tspec _ _ _      -> s == Sspec
+  | Tret  _ _        -> (match s with
+                       | Sret _ -> True
+                       | _ -> False)
+  | Tbind a _ f g    -> (match s with
+                       | Sbind s_f s_g -> 
+                           prog_has_shape' f s_f /\
+                          (forall (x : ts.v a) . prog_has_shape' (g x) s_g)
+                       | _ -> False)
+  | TbindP a _ _ f g -> (match s with
+                       | SbindP s_g ->
+                          (forall (x : a) . prog_has_shape' (g x) s_g)
+                       | _ -> False)
+
+
+type prog_shape (#ts : tys) (#a : ts.t) (t : prog_tree #ts a) =
+  s : shape_tree { prog_has_shape t s }
+
+
+(*** Semantics *)
+
+/// We do not ensure [tree_req f] in the post-condition of [Tbind]. This is equivalent (assuming the
+/// pre-condition, as in [equiv]) but it is simpler for reasoning about some program transformations.
+/// For instance, if one ensures [tree_req f] for the bind, the post-condition of `let x = f in x` is equivalent
+/// to the post-condition of `f` only when the pre-condition holds.
+/// The same holds for [as_requires wp] in the post-condition of [TbindP].
+
+let rec tree_req (#s : tys) (#a : s.t) (t : prog_tree #s a)
+  : Tot pure_pre (decreases t)
+  = match t with
+  | Tnew   _          -> True
+  | Tasrt  p          -> p
+  | Tasum  _          -> True
+  | Tspec  _ pre _    -> pre
+  | Tret   _ _        -> True
+  | Tbind  a b f g    -> tree_req f /\ s.all a (fun (x : s.v a) -> tree_ens f x ==> tree_req (g x))
+  | TbindP a _ wp _ g -> wp (fun x -> tree_req (g x))
+
+and tree_ens (#s : tys) (#a : s.t) (t : prog_tree #s a)
+  : Tot (pure_post (s.v a)) (decreases t)
+  = match t with
+  | Tnew   _          -> fun _  -> True
+  | Tasrt  p          -> fun _(*()*) -> True (* p ?*)
+  | Tasum  p          -> fun _(*()*) -> p
+  | Tspec  a _ post   -> post
+  | Tret   _ x        -> fun r  -> r == s.v_of_r x
+  | Tbind  a _ f g    -> fun y  -> s.ex a (fun (x : s.v a) -> tree_ens f x /\ tree_ens (g x) y)
+  | TbindP a _ wp _ g -> fun y -> (exists (x : a) . as_ensures wp x /\ tree_ens (g x) y)
+
+
+(***** Equivalence *)
+
+let equiv (#s : tys) (#a : s.t) (f g : prog_tree #s a) : prop =
+  (tree_req f <==> tree_req g) /\
+  (tree_req f ==> (forall (x : s.v a) . tree_ens f x <==> tree_ens g x))
+
+
+let equiv_refl (#s : tys) (#a : s.t) (f : prog_tree #s a)
+  : Lemma (equiv f f)
+  = ()
+
+let equiv_sym (#s : tys) (#a : s.t) (f g : prog_tree #s a)
+  : Lemma (requires equiv f g) (ensures equiv g f)
+  = ()
+
+let equiv_trans (#s : tys) (#a : s.t) (f g h : prog_tree #s a)
+  : Lemma (requires equiv f g /\ equiv g h) (ensures equiv f h)
+  = ()
+
+val equiv_Tbind
+      (#s : tys) (#a #b : s.t)
+      (f f' : prog_tree a) (g g' : (x : s.v a) -> prog_tree b)
+      (eq_f : squash (equiv f f')) (eq_g : (x : s.v a) -> squash (equiv (g x) (g' x)))
+  : Lemma (equiv (Tbind a b f g) (Tbind a b f' g'))
+
+val equiv_TbindP
+      (#s : tys) (#a : Type) (#b : s.t) (wp : pure_wp a) (f : unit -> PURE a wp)
+      (g g' : (x : a) -> prog_tree b)
+      (eq_g : (x : a) -> squash (equiv (g x) (g' x)))
+  : Lemma (equiv (TbindP a b wp f g) (TbindP a b wp f g'))
+
+val equiv_Tbind_assoc_Tbind
+      (#s : tys) (#a #b #c : s.t)
+      (f : prog_tree #s a) (g : (x : s.v a) -> prog_tree b) (h : (y : s.v b) -> prog_tree c)
+  : Lemma (equiv (bind (bind f g) h) (bind f (fun x -> bind (g x) h)))
+
+(**) val __end_section_equiv : unit
+
+
+(***** Weakest-precondition *)
+
+let rec tree_wp (#s : tys) (#a : s.t) (t : prog_tree #s a)
+  : Tot (pure_wp (s.v a)) (decreases t)
+  = match t with
+  | Tnew  a           -> MP.as_pure_wp (fun pt -> s.all a (fun (x : s.v a) -> pt x))
+  | Tasrt p           -> MP.as_pure_wp (fun pt -> p /\ (p ==> pt s.emp))
+  | Tasum p           -> MP.as_pure_wp (fun pt -> p ==> pt s.emp)
+  | Tspec a pre post  -> MP.as_pure_wp (fun pt -> pre /\ s.all a (fun (x : s.v a) -> post x ==> pt x))
+  | Tret  _ x         -> MP.as_pure_wp (fun pt -> pt (s.v_of_r x))
+  | Tbind a _ f g     -> MP.elim_pure_wp_monotonicity_forall ();
+                        MP.as_pure_wp (fun pt -> tree_wp f (fun (x : s.v a) -> tree_wp (g x) pt))
+  | TbindP a _ wp _ g -> MP.elim_pure_wp_monotonicity_forall ();
+                        MP.as_pure_wp (fun pt -> wp (fun (x : a) -> tree_wp (g x) pt))
+
+val tree_wp_sound (#s : tys) (#a : s.t) (t : prog_tree #s a) (post : pure_post (s.v a))
+  : Lemma (requires tree_wp t post)
+          (ensures  tree_req t /\ (forall (x : s.v a) . tree_ens t x ==> post x))
+
+
+(*** Returns elimination *)
+
+/// This transformation aims to eliminate the [Tret] introduced by previous transformations (Steel.Repr.M ->
+/// Steel.Repr.ST -> Steel.Repr.Fun).
+/// We do not try to handle all possible simplifications but rather to have a transformation that works in our cases.
+/// It currently performs a binders flattening (similar to the one on Steel.Repr.ST), with a special handling of
+/// returns in order to be able to push them below [TbindP].
+/// We only simplify the returns marked with [smp_ret] in the shape, that is, the returns introduced by the
+/// transformations. (TODO: test)
+
+noeq
+type elim_returns_k (st : tys) (a a1 : st.t) =
+  | ERetKfun : (k : st.v a -> st.v a1) -> elim_returns_k st a a1
+  | ERetKtrm : (k : st.v a -> prog_tree #st a1) -> elim_returns_k st a a1
+
+let elim_returns_k_ret (#st : tys) (#a #a1 : st.t) (f : st.v a -> st.v a1) (x : st.v a)
+  : prog_tree #st a1
+  = Tret a1 (st.r_of_v (f x))
+
+let elim_returns_k_trm (#st : tys) (#a #a1 : st.t) (k : elim_returns_k st a a1)
+  : st.v a -> prog_tree #st a1
+  = match k with
+  | ERetKfun kf -> elim_returns_k_ret kf
+  | ERetKtrm kt -> kt
+
+let rec elim_returns
+      (#st : tys) (#a : st.t) (t : prog_tree u#t u#v u#r u#a #st a) (s : prog_shape t)
+  : Tot (prog_tree u#t u#v u#r u#a #st a) (decreases %[t; 1])
+  = elim_returns_aux t s (ERetKfun id)
+
+and elim_returns_aux
+      (#st : tys) (#a : st.t) (t : prog_tree u#t u#v u#r u#a #st a) (s : prog_shape t)
+      (#a1 : st.t) (k : elim_returns_k st a a1)
+  : Tot (prog_tree u#t u#v u#r u#a #st a1) (decreases %[t; 0])
+  = match t with
+  | Tnew _ | Tasrt _ | Tasum _ | Tspec _ _ _ ->
+         Tbind _ _ t (elim_returns_k_trm k)
+  | Tret a x ->
+         let Sret smp_ret = s in
+         if smp_ret then elim_returns_k_trm k (st.v_of_r x)
+         else begin match k with
+         | ERetKfun kf -> Tret a1 (st.r_of_v (kf (st.v_of_r x)))
+         | ERetKtrm kt -> Tbind _ _ (Tret a x) kt
+         end
+  | Tbind a b f g ->
+         let Sbind s_f s_g = s in
+         begin match s_g, k with
+         | Sret true, ERetKfun kf ->
+               let k1 (x : st.v a) = kf (st.v_of_r (Tret?.x (g x))) in
+               elim_returns_aux f s_f (ERetKfun k1)
+         | _ -> let k1 (x : st.v a) = elim_returns_aux (g x) s_g k in
+               elim_returns_aux f s_f (ERetKtrm k1)
+         end
+  | TbindP a b wp f g ->
+         let SbindP s_g = s in
+         begin match k with
+         | ERetKfun kf -> TbindP a a1 wp f (fun (x : a) -> elim_returns_aux (g x) s_g (ERetKfun kf))
+         | ERetKtrm kt -> Tbind b a1 (TbindP a b wp f (fun (x : a) -> elim_returns (g x) s_g)) kt
+         end
+
+val elim_returns_equiv
+      (#st : tys) (#a : st.t) (t : prog_tree u#t u#v u#r u#a #st a) (s : prog_shape t)
+  : Lemma (equiv (elim_returns t s) t)
+
+val elim_returns_equiv_aux
+      (#st : tys) (#a : st.t) (t : prog_tree u#t u#v u#r u#a #st a) (s : prog_shape t)
+      (#a1 : st.t) (k : elim_returns_k st a a1)
+  : Lemma (equiv (elim_returns_aux t s k) (Tbind a a1 t (elim_returns_k_trm k)))
